nola/iris/fborrow.v
@@ -1,196 +1,178 @@
 (** * Fractured borrows *)
 
-From nola.iris Require Export dinv_deriv borrow_deriv.
-From nola.util Require Import tagged.
+From nola.iris Require Export dinv borrow.
 From iris.bi Require Export lib.fractional.
 From iris.proofmode Require Import proofmode.
-Import ProdNotation iPropAppNotation ModwNotation LftNotation DsemNotation.
+Import ProdNotation iPropAppNotation ModwNotation LftNotation.
 
-Implicit Type (α : lft) (q : Qp) (Σ : gFunctors) (FML : oFunctor) (FM : ofe).
+Implicit Type (α : lft) (q : Qp) (Σ : gFunctors) (FML : oFunctor) (JUDG : ofe).
 
 (** Formula for fractured borrows *)
-Variant fborrow_fml_id := .
-Definition fborrow_fmlOF FML : oFunctor :=
-  leibnizO (tagged fborrow_fml_id lft) * (Qp -d> FML).
+Definition fborrow_fmlOF FML : oFunctor := leibnizO lft * (Qp -d> FML).
 
 (** Ghost state for fractured borrows *)
 Class fborrowGpreS FML Σ : Type :=
-  fborrowGpreS_dinv :: dinvGpreS (fborrow_fmlOF FML) Σ.
-Class fborrowGS FML Σ : Type := fborrowGS_dinv :: dinvGS (fborrow_fmlOF FML) Σ.
+  fborrowGpreS_dinv : dinvGpreS (fborrow_fmlOF FML) Σ.
+Local Existing Instance fborrowGpreS_dinv.
+Class fborrowGS FML Σ : Type := fborrowGS_dinv : dinvGS (fborrow_fmlOF FML) Σ.
+Local Existing Instance fborrowGS_dinv.
 Definition fborrowΣ FML `{!oFunctorContractive FML} :=
   dinvΣ (fborrow_fmlOF FML).
 #[export] Instance subG_fborrowΣ
   `{!oFunctorContractive FML, !subG (fborrowΣ FML) Σ} : fborrowGpreS FML Σ.
 Proof. solve_inG. Qed.
 
-Section fborrow_wsat.
-  Context `{!fborrowGS FML Σ, !borrowGS FML Σ, !bupdJ (FML $oi Σ) JUDG}.
-  Implicit Type (Φx : Qp -d> FML $oi Σ) (δ : JUDG -n> iProp Σ).
+Section fborrow.
+  Context `{!fborrowGS FML Σ, !borrowGS FML Σ}.
+  Implicit Type (Φx : Qp -d> FML $oi Σ).
+
+  (** [fbor_tok]: Fractured borrower token *)
+  Local Definition fbor_tok_def α Φx : iProp Σ :=
+    ∃ α', α ⊑□ α' ∗ dinv_tok (α', Φx).
+  Local Lemma fbor_tok_aux : seal fbor_tok_def. Proof. by eexists. Qed.
+  Definition fbor_tok := fbor_tok_aux.(unseal).
+  Local Lemma fbor_tok_unseal : fbor_tok = fbor_tok_def.
+  Proof. exact: seal_eq. Qed.
+
+  (** [fbor_tok] is persistent *)
+  #[export] Instance fbor_tok_persistent {α Φx} : Persistent (fbor_tok α Φx).
+  Proof. rewrite fbor_tok_unseal. exact _. Qed.
+  (** [fbor_tok] is timeless for discrete formulas *)
+  #[export] Instance fbor_tok_timeless {α} `{!Discrete Φx} :
+    Timeless (fbor_tok α Φx).
+  Proof. rewrite fbor_tok_unseal. exact _. Qed.
+  (** [fbor_tok] is non-expansive *)
+  #[export] Instance fbor_tok_ne {α} : NonExpansive (fbor_tok α).
+  Proof.
+    rewrite fbor_tok_unseal /fbor_tok_def=> ????. do 4 f_equiv. solve_proper.
+  Qed.
+  #[export] Instance fbor_tok_proper {α} : Proper ((≡) ==> (≡)) (fbor_tok α).
+  Proof. apply ne_proper, _. Qed.
 
   (** [fborrow_sem]: Semantics for [fborrow_fmlOF] *)
-  Definition fborrow_sem δ : fborrow_fmlOF FML $oi Σ → iProp Σ :=
-    λ '(Tagged α, Φx), (∃ q, bor δ α (Φx q))%I.
+  Definition fborrow_sem : fborrow_fmlOF FML $oi Σ → iProp Σ :=
+    λ '(α, Φx), (∃ q, bor_tok α (Φx q))%I.
   (** [fborrow_sem] is non-expansive *)
-  #[export] Instance fborrow_sem_ne {δ} : NonExpansive (fborrow_sem δ).
+  #[export] Instance fborrow_sem_ne : NonExpansive fborrow_sem.
   Proof. move=> ?[??][??][/=/leibniz_equiv_iff<- ?]. solve_proper. Qed.
-  (** [Dsem] for [fborrow_fmlOF] *)
-  #[export] Instance fborrow_dsem :
-    Dsem JUDG (fborrow_fmlOF FML $oi Σ) (iProp Σ) := DSEM fborrow_sem _.
 
   (** [fborrow_wsat]: World satisfaction for fractured borrows *)
-  Local Definition fborrow_wsat_def δ : iProp Σ := dinv_wsat (fborrow_dsem δ).
+  Local Definition fborrow_wsat_def : iProp Σ := dinv_wsat fborrow_sem.
   Local Lemma fborrow_wsat_aux : seal fborrow_wsat_def. Proof. by eexists. Qed.
   Definition fborrow_wsat := fborrow_wsat_aux.(unseal).
   Local Lemma fborrow_wsat_unseal : fborrow_wsat = fborrow_wsat_def.
   Proof. exact: seal_eq. Qed.
-End fborrow_wsat.
-Notation fborrow_wsatd := (fborrow_wsat der).
+
+  (** [fborrow_wsat] is timeless when all formulas are discrete *)
+  #[export] Instance fborrow_wsat_timeless `{!OfeDiscrete (FML $oi Σ)} :
+    Timeless fborrow_wsat.
+  Proof.
+    rewrite fborrow_wsat_unseal. apply: dinv_wsat_timeless. case. exact _.
+  Qed.
+End fborrow.
 
 (** Allocate [fborrow_wsat] *)
-Lemma fborrow_wsat_alloc `{!borrowGS FML Σ, !fborrowGpreS FML Σ,
-  !bupdJ (FML $oi Σ) JUDG} :
-  ⊢ |==> ∃ _ : fborrowGS FML Σ, ∀ δ, fborrow_wsat δ.
+Lemma fborrow_wsat_alloc `{!borrowGS FML Σ, !fborrowGpreS FML Σ} :
+  ⊢ |==> ∃ _ : fborrowGS FML Σ, fborrow_wsat.
 Proof.
-  iMod dinv_wsat_alloc as (?) "→W". iModIntro. iExists _. iIntros (?).
+  iMod dinv_wsat_alloc as (?) "→W". iModIntro. iExists _.
   rewrite fborrow_wsat_unseal. iApply "→W". iApply ne_internal_ne.
 Qed.
 
-(** [fborrowJ]: Judgment for [fborrow] registered *)
-Notation fborrowJ FML JUDG Σ := (dinvJ (fborrow_fmlOF FML $oi Σ) JUDG).
-(** [fborrowJS]: Judgment semantics for [fborrow] registered *)
-Notation fborrowJS FML JUDG Σ := (dinvJS (fborrow_fmlOF FML) JUDG Σ).
+Section fborrow.
+  Context `{!borrowGS FML Σ, !fborrowGS FML Σ, !ModUpd (PROP:=iProp Σ) M,
+    !ModBUpd M}.
 
-Section fbor.
-  Context `{!borrowGS FML Σ, !fborrowJ FML JUDG Σ}.
-  Implicit Type (δ : JUDG -n> iProp Σ) (Φx : Qp -d> FML $oi Σ).
+  (** Modify the lifetime of [fbor_tok] *)
+  Lemma fbor_tok_lft {α β Φx} : β ⊑□ α -∗ fbor_tok α Φx -∗ fbor_tok β Φx.
+  Proof.
+    rewrite fbor_tok_unseal. iIntros "#⊑ (% & #⊑' & $)".
+    by iApply lft_sincl_trans.
+  Qed.
 
-  (** [fbor]: Relaxed fractured borrower *)
-  Local Definition fbor_def δ α Φx : iProp Σ :=
-    ∃ α', α ⊑□ α' ∗ dinv δ (Tagged α' : leibnizO _, Φx).
-  Local Lemma fbor_aux : seal fbor_def. Proof. by eexists. Qed.
-  Definition fbor := fbor_aux.(unseal).
-  Local Lemma fbor_unseal : fbor = fbor_def. Proof. exact: seal_eq. Qed.
+  (** Allocate [fbor_tok] from [bor_tok] *)
+  Lemma fbor_tok_alloc {α} Φx q :
+    bor_tok α (Φx q) =[fborrow_wsat]=∗ fbor_tok α Φx.
+  Proof.
+    iIntros "b". rewrite fbor_tok_unseal fborrow_wsat_unseal.
+    iMod (dinv_tok_alloc (FML:=fborrow_fmlOF _) (α, Φx) with "[b]")
+      as "$"=>/=; [by iExists _|].
+    iModIntro. iApply lft_sincl_refl.
+  Qed.
 
-  (** [fbor] is persistent *)
-  #[export] Instance fbor_persistent {δ α Φx} : Persistent (fbor δ α Φx).
-  Proof. rewrite fbor_unseal. exact _. Qed.
-  (** [fbor] is non-expansive *)
-  #[export] Instance fbor_ne {δ α} : NonExpansive (fbor δ α).
-  Proof. rewrite fbor_unseal /fbor_def=> ????. do 4 f_equiv. solve_proper. Qed.
-  #[export] Instance fbor_proper {δ α} : Proper ((≡) ==> (≡)) (fbor δ α).
-  Proof. apply ne_proper, _. Qed.
-End fbor.
-Notation fbord := (fbor der).
-
-Section fbor.
-  Context `{!borrowGS FML Σ, !bupdJ (FML $oi Σ) JUDG, !fborrowGS FML Σ,
-    !fborrowJ FML JUDG Σ, !Dsem JUDG (FML $oi Σ) (iProp Σ),
-    !Jsem JUDG (iProp Σ), !bupdJS (FML $oi Σ) JUDG (iProp Σ),
-    !fborrowJS FML JUDG Σ, !ModUpd (PROP:=iProp Σ) M, !ModBUpd M}.
-
-  (** Access the content of [fbord] under the fractionality of [Φx] *)
-  Lemma fbord_acc_bord {α Φx r} :
-    Fractional (λ q, ⟦ Φx q ⟧) →
-    r.[α] -∗ fbord α Φx -∗ modw M (fborrow_wsatd ∗ borrow_wsat M ⟦⟧)
+  (** Access the content of [fbor_tok] under the fractionality of [Φx] *)
+  Lemma fbor_tok_acc_bor_tok {α Φx r sm} :
+    Fractional (λ q, sm (Φx q)) →
+    r.[α] -∗ fbor_tok α Φx -∗ modw M (fborrow_wsat ∗ borrow_wsat M sm)
       (∃ q, r.[α] ∗ bor_tok α (Φx q)).
   Proof.
-    rewrite fbor_unseal. iIntros (frac) "α (%α' & #⊑ & f) [Wf Wb]".
+    rewrite fbor_tok_unseal. iIntros (frac) "α (%α' & #⊑ & f) [Wf Wb]".
     rewrite fborrow_wsat_unseal.
-    iDestruct (dinvd_acc (FML:=fborrow_fmlOF _) with "f Wf") as "/=[[%q b] cl]".
+    iDestruct (dinv_tok_acc (FML:=fborrow_fmlOF _) with "f Wf")
+      as "/=[[%q b] cl]".
     iMod (lft_sincl_live_acc with "⊑ α") as (?) "[α' →α]".
-    iMod (bord_open with "α' b Wb") as "(Wb & o & Φx)".
-    iMod (obord_subdiv [Φx (q/2)%Qp; Φx (q/2)%Qp] α' with "[] o [Φx] [] Wb")
+    iMod (bor_tok_open with "α' b Wb") as "(Wb & o & Φx)".
+    iMod (obor_tok_subdiv [Φx (q/2)%Qp; Φx (q/2)%Qp] α' with "[] o [Φx] [] Wb")
       as "($ & α' & _ & b & b' & _)"=>/=.
     { iApply lft_sincl_refl. }
     { rewrite -{1}(Qp.div_2 q) frac. iDestruct "Φx" as "[$$]". }
     { rewrite -{3}(Qp.div_2 q) frac. by iIntros "_ [$[$ _]]". }
     iModIntro. iDestruct ("→α" with "α'") as "$".
-    iDestruct (bor_tok_lft with "⊑ b") as "$". iApply "cl". iExists _.
-    by rewrite -bor_tok_bor.
+    iDestruct (bor_tok_lft with "⊑ b") as "$". iApply "cl". by iExists _.
   Qed.
-  Lemma fbord_acc {α Φx r} :
-    Fractional (λ q, ⟦ Φx q ⟧) →
-    r.[α] -∗ fbord α Φx -∗ modw M (fborrow_wsatd ∗ borrow_wsat M ⟦⟧)
-      (∃ q, ⟦ Φx q ⟧ ∗ (⟦ Φx q ⟧ =[borrow_wsat M ⟦⟧]=∗ r.[α])).
+  Lemma fbor_tok_acc {α Φx r sm} :
+    Fractional (λ q, sm (Φx q)) →
+    r.[α] -∗ fbor_tok α Φx -∗ modw M (fborrow_wsat ∗ borrow_wsat M sm)
+      (∃ q, sm (Φx q) ∗ (sm (Φx q) =[borrow_wsat M sm]=∗ r.[α])).
   Proof.
-    iIntros (frac) "α f". iMod (fbord_acc_bord with "α f") as (?) "[α b]"=>//.
-    iIntros "[$ Wb]". iMod (bor_tok_open with "α b Wb") as "/=($ & o & $)".
-    iIntros "!> Φx". by iMod (obor_tok_close (M:=M) with "o Φx") as "[$ _]".
+    iIntros (frac) "α f".
+    iMod (fbor_tok_acc_bor_tok with "α f") as (?) "[α b]"=>//. iIntros "[$ Wb]".
+    iMod (bor_tok_open with "α b Wb") as "/=($ & o & $)". iIntros "!> Φx".
+    by iMod (obor_tok_close (M:=M) with "o Φx") as "[$ _]".
   Qed.
-
-  (** Modify the lifetime of [fbor] *)
-  Lemma fbor_lft {δ α β Φx} : β ⊑□ α -∗ fbor δ α Φx -∗ fbor δ β Φx.
-  Proof.
-    rewrite fbor_unseal. iIntros "#⊑ (% & #⊑' & $)". by iApply lft_sincl_trans.
-  Qed.
-
-  Context `{!Deriv (JUDG:=JUDG) ih δ}.
-
-  (** Allocate [fbor] from [bor] *)
-  Lemma fbor_alloc {α} Φx q : bor δ α (Φx q) =[fborrow_wsat δ]=∗ fbor δ α Φx.
-  Proof.
-    iIntros "b". rewrite fbor_unseal fborrow_wsat_unseal.
-    iMod (dinv_alloc (FML:=fborrow_fmlOF _) (Tagged α, Φx) with "[b]")
-      as "$"=>/=; [by iExists _|].
-    iModIntro. iApply lft_sincl_refl.
-  Qed.
-
-  (** Convert the body of [fbor] *)
-  Lemma fbor_to {α Φx Ψx} :
-    □ (∀ q δ', ⌜Deriv ih δ'⌝ → ⌜ih δ'⌝ → ⟦ Φx q ⟧(δ') ==∗ ⟦ Ψx q ⟧(δ')) -∗
-    □ (∀ q δ', ⌜Deriv ih δ'⌝ → ⌜ih δ'⌝ → ⟦ Ψx q ⟧(δ') ==∗ ⟦ Φx q ⟧(δ')) -∗
-    fbor δ α Φx -∗ fbor δ α Ψx.
-  Proof.
-    iIntros "#ΦΨ #ΨΦ". rewrite fbor_unseal. iIntros "(% & $ & i)".
-    iApply (dinv_iff (FML:=fborrow_fmlOF _) with "[] i"). iIntros (????) "!>/=".
-    iSplit; iIntros "[%q b]"; iExists q;
-      (iApply (bor_to (ih:=ih) with "[] [] b");
-        iIntros "!>" (????); by [iApply "ΦΨ"|iApply "ΨΦ"]).
-  Qed.
-End fbor.
+End fborrow.
 
 (** ** Constructor *)
 
 From nola.iris Require Import cif.
 
-(** [fborCT]: Constructor *)
-Variant fborCT_id := .
-Definition fborCT :=
-  Cifcon fborCT_id lft (λ _, Empty_set) (λ _, Qp) (λ _, unitO) _.
-(** [fborC]: [fborCT] registered *)
-Notation fborC := (inC fborCT).
+(** [fbor_tokCT]: Constructor *)
+Variant fbor_tokCT_id := .
+Definition fbor_tokCT :=
+  Cifcon fbor_tokCT_id lft (λ _, Empty_set) (λ _, Qp) (λ _, unitO) _.
+(** [fbor_tokC]: [fbor_tokCT] registered *)
+Notation fbor_tokC := (inC fbor_tokCT).
 
-Section fborC.
-  Context `{!fborC CON} {Σ}.
+Section fbor_tokC.
+  Context `{!fbor_tokC CON} {Σ}.
   Implicit Type Φx : Qp -d> cif CON Σ.
-  (** [cif_fbor]: Formula for [fbor] *)
-  Definition cif_fbor α Φx : cif CON Σ :=
-    cif_in fborCT α nullary Φx ().
-  (** [cif_fbor] is non-expansive *)
-  #[export] Instance cif_fbor_ne {α} : NonExpansive (cif_fbor α).
+  (** [cif_fbor_tok]: Formula for [fbor_tok] *)
+  Definition cif_fbor_tok α Φx : cif CON Σ :=
+    cif_in fbor_tokCT α nullary Φx ().
+  (** [cif_fbor_tok] is non-expansive *)
+  #[export] Instance cif_fbor_tok_ne {α} : NonExpansive (cif_fbor_tok α).
   Proof. solve_proper. Qed.
-  #[export] Instance cif_fbor_proper {α} : Proper ((≡) ==> (≡)) (cif_fbor α).
+  #[export] Instance cif_fbor_tok_proper {α} :
+    Proper ((≡) ==> (≡)) (cif_fbor_tok α).
   Proof. apply ne_proper, _. Qed.
-  (** [cif_fbor] is productive *)
-  #[export] Instance cif_bor_productive {α} : Productive (cif_fbor α).
+  (** [cif_fbor_tok] is productive *)
+  #[export] Instance cif_fbor_tok_productive {α} : Productive (cif_fbor_tok α).
   Proof. move=> ????. by apply cif_in_preserv_productive. Qed.
 
-  Context `{!dinvJ (cifO CON Σ) JUDG, !borrowGS (cifOF CON) Σ,
-    !fborrowJ (cifOF CON) JUDG Σ}.
-  #[export] Program Instance fborCT_ecsem : Ecsem fborCT CON JUDG Σ :=
-    ECSEM (λ _ δ α _ Φx _, fbor δ α Φx) _.
+  Context `{!borrowGS (cifOF CON) Σ, !fborrowGS (cifOF CON) Σ} {JUDG}.
+  #[export] Program Instance fbor_tokCT_ecsem : Ecsem fbor_tokCT CON JUDG Σ :=
+    ECSEM (λ _ _ α _ Φx _, fbor_tok α Φx) _.
   Next Obligation. solve_proper. Qed.
-End fborC.
-(** [fborCS]: Semantics of [fborCT] registered *)
-Notation fborCS := (inCS fborCT).
+End fbor_tokC.
+(** [fbor_tokCS]: Semantics of [fbor_tokCT] registered *)
+Notation fbor_tokCS := (inCS fbor_tokCT).
 
-(** Reify [fbor] *)
-Section fborC.
-  Context `{!Csem CON JUDG Σ, !Jsem JUDG (iProp Σ), !dinvJ (cifO CON Σ) JUDG,
-    !borrowGS (cifOF CON) Σ, !fborrowJ (cifOF CON) JUDG Σ, !fborC CON,
-    !fborCS CON JUDG Σ}.
+(** Reify [fbor_tok] *)
+Section fbor_tokC.
+  Context `{!fbor_tokC CON, !Csem CON JUDG Σ, !Jsem JUDG (iProp Σ),
+    !borrowGS (cifOF CON) Σ, !fborrowGS (cifOF CON) Σ, !fbor_tokCS CON JUDG Σ}.
 
-  #[export] Program Instance fbor_as_cif {α Φx} :
-    AsCif CON (λ δ, fbor δ α Φx) := AS_CIF (cif_fbor α Φx) _.
+  #[export] Program Instance fbor_tok_as_cif {α Φx} :
+    AsCif CON (λ _, fbor_tok α Φx) := AS_CIF (cif_fbor_tok α Φx) _.
   Next Obligation. move=>/= >. by rewrite sem_cif_in. Qed.
-End fborC.
+End fbor_tokC.
